omni/SepLogicSmall.v
@@ -1,0 +1,267 @@
+(****************************************************************
+* Imperative Lambda-calculus                                    *
+* Separation Logic on Small-Step                                *
+*****************************************************************)
+
+Set Implicit Arguments.
+Require Export SepLogicCommon Small.
+
+Implicit Types f : var.
+Implicit Types b : bool.
+Implicit Types p : loc.
+Implicit Types n : int.
+Implicit Types v w r vf vx : val.
+Implicit Types t : trm.
+Implicit Types s : state.
+Implicit Types h : heap.
+Implicit Types H : hprop.
+Implicit Types Q : val->hprop.
+
+
+(* ########################################################### *)
+(* ########################################################### *)
+(* ########################################################### *)
+(** * Proof of the Frame Property for the Small-Step-Based [stepsinto] Relation *)
+
+Hint Constructors step.
+
+Lemma stepsinto_frame : forall h1 h2 t Q,
+  stepsinto h1 t Q ->
+  Fmap.disjoint h1 h2 ->
+  stepsinto (h1 \u h2) t (Q \*+ (= h2)).
+Proof using.
+  introv M HD. gen h2. induction M; intros.
+  { applys stepsinto_val. applys* hstar_intro. }
+  { rename H into M1, H0 into M2, H1 into IH2.
+    applys stepsinto_step.
+    { unfolds reducible. clear M2 IH2. destruct M1 as (s'&t'&R).
+      induction R; tryfalse; try solve [ do 2 esplit; constructors* ].
+      { forwards* (s'&t'&R'): IHR. }
+      { lets (p'&F&_): exists_fresh null (Fmap.union s h2). do 2 esplit.
+        applys step_ref v p'. eauto. }
+      { do 2 esplit. applys step_get. applys* Fmap.indom_union_l. }
+      { do 2 esplit. applys step_set. applys* Fmap.indom_union_l. }
+      { do 2 esplit. applys step_free. applys* Fmap.indom_union_l. } }
+    { introv R. cuts (s1'&E'&D'&R'):
+        (exists s1', s' = s1' \u h2 /\ Fmap.disjoint s1' h2 /\ step s t s1' t').
+      { subst. applys* IH2. }
+      clear M2 IH2.
+      gen_eq su: (s \u h2). gen s.
+      unfolds reducible. induction R; intros; subst; eauto.
+      { destruct M1 as (s0&t0&R0).
+        rename R into R1. forwards* (s1'&E&D&R1'): IHR s.
+        { inverts R0. { eauto. } { inverts R1. } } }
+      { rename H into D. rewrite Fmap.indom_union_eq in D. rew_logic in D.
+        destruct D as (D1&D2). esplit. splits.
+        { rewrite* Fmap.update_union_not_r. }
+        { applys* Fmap.disjoint_update_not_r. }
+        { eauto. } }
+      { destruct M1 as (se&te&Re). inverts Re; tryfalse.
+        rewrite* Fmap.read_union_l. }
+      { destruct M1 as (se&te&Re). inverts Re; tryfalse. esplit. splits.
+        { rewrite* Fmap.update_union_l. }
+        { applys* Fmap.disjoint_update_l. }
+        { eauto. } }
+      { destruct M1 as (se&te&Re). inverts Re; tryfalse. esplit. splits.
+        { rewrite* remove_disjoint_union_l. }
+        { applys* Fmap.disjoint_remove_l. }
+        { eauto. } } } }
+Qed.
+
+
+(* ########################################################### *)
+(* ########################################################### *)
+(* ########################################################### *)
+(** * Deriving Big-Step Evaluation Rules for [stepsinto] *)
+
+Lemma stepsinto_fix : forall s f x t1 Q,
+  Q (val_fix f x t1) s ->
+  stepsinto s (trm_fix f x t1) Q.
+Proof using.
+  introv M. applys stepsinto_step.
+  { do 2 esplit. constructor. }
+  { introv R. inverts R. { applys stepsinto_val. applys M. } }
+Qed.
+
+Lemma stepsinto_app_fix : forall s f x v1 v2 t1 Q,
+  v1 = val_fix f x t1 ->
+  stepsinto s (subst x v2 (subst f v1 t1)) Q ->
+  stepsinto s (trm_app v1 v2) Q.
+Proof using.
+  introv E M. applys stepsinto_step.
+  { do 2 esplit. applys* step_app_fix. }
+  { introv R. invert R; try solve [intros; false].
+    introv -> -> -> -> -> R. inverts E. applys M. }
+Qed.
+
+Lemma stepsinto_let : forall s x t1 t2 Q1 Q,
+  stepsinto s t1 Q1 ->
+  (forall s1 v1, Q1 v1 s1 -> stepsinto s1 (subst x v1 t2) Q) ->
+  stepsinto s (trm_let x t1 t2) Q.
+Proof using.
+  introv M1 M2. gen_eq Q1': Q1.
+  induction M1; intros; subst.
+  { apply stepsinto_step.
+    { do 2 esplit. applys step_let. }
+    { introv R. inverts R as R'. { inverts R'. } applys* M2. } }
+  { rename t into t1, H1 into IH.
+    destruct H as (s'&t'&RE). applys stepsinto_step.
+    { do 2 esplit. constructors. applys RE. }
+    { introv R. inverts R as R'.
+      { applys* IH R' M2. }
+      { false. inverts RE. } } }
+Qed.
+
+Lemma stepsinto_if : forall s b t1 t2 Q,
+  stepsinto s (if b then t1 else t2) Q ->
+  stepsinto s (trm_if b t1 t2) Q.
+Proof using.
+  introv M. applys stepsinto_step.
+  { do 2 esplit. constructors*. }
+  { introv R. inverts R; tryfalse. { applys M. } }
+Qed.
+
+
+(* ########################################################### *)
+(* ########################################################### *)
+(* ########################################################### *)
+(** * Construction of Separation Logic *)
+
+(* ########################################################### *)
+(** ** Definition of Separation Logic triples *)
+
+Definition triple (t:trm) (H:hprop) (Q:val->hprop) : Prop :=
+  forall s, H s -> stepsinto s t Q.
+
+(* ########################################################### *)
+(** ** Structural Rules *)
+
+Lemma triple_conseq : forall t H' Q' H Q,
+  triple t H' Q' ->
+  H ==> H' ->
+  Q' ===> Q ->
+  triple t H Q.
+Proof using. unfolds triple. introv M MH MQ HF. applys* stepsinto_conseq. Qed.
+
+Lemma triple_frame : forall t H Q H',
+  triple t H Q ->
+  triple t (H \* H') (Q \*+ H').
+Proof.
+  introv M. intros h HF. lets (h1&h2&M1&M2&MD&MU): (rm HF).
+  subst. specializes M M1. applys stepsinto_conseq.
+  { applys stepsinto_frame M MD. } { xsimpl. intros h' ->. applys M2. }
+Qed.
+
+Lemma triple_hexists : forall t (A:Type) (J:A->hprop) Q,
+  (forall (x:A), triple t (J x) Q) ->
+  triple t (hexists J) Q.
+Proof using. introv M. intros h (x&Hh). applys M Hh. Qed.
+
+Lemma triple_hpure : forall t (P:Prop) H Q,
+  (P -> triple t H Q) ->
+  triple t (\[P] \* H) Q.
+Proof using.
+  introv M. intros h (h1&h2&M1&M2&D&U). destruct M1 as (M1&HP).
+  inverts HP. subst. rewrite Fmap.union_empty_l. applys~ M.
+Qed.
+
+
+(* ########################################################### *)
+(** ** Reasoning Rules for Terms *)
+
+Lemma triple_val : forall v H Q,
+  H ==> Q v ->
+  triple (trm_val v) H Q.
+Proof using. introv M Hs. applys* stepsinto_val. Qed.
+
+Lemma triple_fix : forall f x t1 H Q,
+  H ==> Q (val_fix f x t1) ->
+  triple (trm_fix f x t1) H Q.
+Proof using. introv M Hs. applys* stepsinto_fix. Qed.
+
+Lemma triple_if : forall (b:bool) t1 t2 H Q,
+  triple (if b then t1 else t2) H Q ->
+  triple (trm_if b t1 t2) H Q.
+Proof using. introv M Hs. applys* stepsinto_if. Qed.
+
+Lemma triple_app_fix : forall v1 v2 f x t1 H Q,
+  v1 = val_fix f x t1 ->
+  triple (subst x v2 (subst f v1 t1)) H Q ->
+  triple (trm_app v1 v2) H Q.
+Proof using. introv E M Hs. applys* stepsinto_app_fix. Qed.
+
+Lemma triple_let : forall x t1 t2 Q1 H Q,
+  triple t1 H Q1 ->
+  (forall v1, triple (subst x v1 t2) (Q1 v1) Q) ->
+  triple (trm_let x t1 t2) H Q.
+Proof using. unfolds triple. introv M1 M2 Hs. applys* stepsinto_let. Qed.
+
+
+(* ########################################################### *)
+(** ** Specification of Primitive Operations *)
+
+Lemma triple_div : forall n1 n2,
+  n2 <> 0 ->
+  triple (val_div n1 n2)
+    \[]
+    (fun r => \[r = val_int (Z.quot n1 n2)]).
+Proof using.
+  introv Hn2 Hs. applys* stepsinto_step.
+  { introv R. inverts R. applys* stepsinto_val. hnfs*. }
+Qed.
+
+Lemma triple_rand : forall n,
+  n > 0 ->
+  triple (val_rand n)
+    \[]
+    (fun r => \[exists n1, r = val_int n1 /\ 0 <= n1 < n]).
+Proof using.
+  introv Hn2 Hs. applys* stepsinto_step.
+  { exists s 0. constructors. math. }
+  { introv R. inverts R; tryfalse. applys* stepsinto_val. hnfs*. }
+Qed.
+
+Lemma triple_ref : forall v,
+  triple (val_ref v)
+    \[]
+    (fun r => \exists p, \[r = val_loc p] \* p ~~> v).
+Proof using.
+  intros. intros s1 K. applys* stepsinto_step.
+  { forwards~ (p&D&N): (exists_fresh null s1). do 2 esplit. applys* step_ref. }
+  { introv R. inverts R; tryfalse. applys stepsinto_val.
+    inverts K. rewrite Fmap.update_empty. exists p.
+    rewrite hstar_hpure_l. split*. hnfs*. }
+Qed.
+
+Lemma triple_get : forall v p,
+  triple (val_get p)
+    (p ~~> v)
+    (fun r => \[r = v] \* (p ~~> v)).
+Proof using.
+  intros. intros s K. inverts K. applys* stepsinto_step.
+  { do 2 esplit. applys* step_get. applys* Fmap.indom_single. }
+  { introv R. inverts R; tryfalse. applys stepsinto_val.
+    rewrite hstar_hpure_l. split*. rewrite* Fmap.read_single. hnfs*. }
+Qed.
+
+Lemma triple_set : forall w p v,
+  triple (val_set (val_loc p) v)
+    (p ~~> w)
+    (fun r => (p ~~> v)).
+Proof using.
+  intros. intros s1 K. inverts K. applys* stepsinto_step.
+  { do 2 esplit. applys* step_set. applys* Fmap.indom_single. }
+  { introv R. inverts R; tryfalse. applys stepsinto_val.
+    rewrite Fmap.update_single. hnfs*. }
+Qed.
+
+Lemma triple_free : forall p v,
+  triple (val_free (val_loc p))
+    (p ~~> v)
+    (fun r => \[]).
+Proof using.
+  intros. intros s1 K. inverts K. applys* stepsinto_step.
+  { do 2 esplit. applys* step_free. applys* Fmap.indom_single. }
+  { introv R. inverts R; tryfalse. applys stepsinto_val.
+    rewrite* Fmap.remove_single. hnfs*. }
+Qed.
